new_stack done (invariant tweak)

theories/iris/examples/stack/function/push.v
@@ -15,395 +15,411 @@ Close Scope byte_scope.
 
 
 Section stack.
-
- Context `{!wasmG Σ}. 
-
- 
-Section code.
-
-Definition push :=
-  validate_stack 1 ++ 
-  [
-    BI_get_local 1 ;
-    BI_load T_i32 None N.zero N.zero ;
-    BI_tee_local 2 ;
-    i32const 65536;
-    BI_binop T_i32 (Binop_i (BOI_rem SX_U)) ;
-    BI_if (Tf [] []) [] [BI_unreachable] ;
-    BI_get_local 2 ;
-    BI_get_local 0 ;
-    BI_store T_i32 None N.zero N.zero ;
-    BI_get_local 1 ;
-    BI_get_local 2 ;
-    i32const 4 ;
-    BI_binop T_i32 (Binop_i BOI_add) ;
-    BI_store T_i32 None N.zero N.zero
-  ].
-
-End code.
-
-
-
-Section specs.
-
-Lemma push_not_full v (s: list i32) f E:
-  (two16 | v)%Z ->  
-  (length s < two14 - 1)%Z ->
-  ↪[frame] f ⊢
-  WP [AI_basic (BI_const (value_of_int (v + 4 + length s * 4))); AI_basic (i32const 65536);
-     AI_basic (BI_binop T_i32 (Binop_i (BOI_rem SX_U))); AI_basic (BI_if (Tf [] []) [] [BI_unreachable])] @ E
-     {{ w, ⌜ w = immV [] ⌝ ∗ ↪[frame] f }}.
-Proof.
-  move => Hdiv Hsize.
-  iIntros "Hf".
-  rewrite separate3.
-  iApply wp_seq.
-  instantiate (1 := λ w, (⌜ w = immV [ _ ]⌝ ∗ ↪[frame] f)%I).
-  iSplitR; first by iIntros "(%H & _)".
-  iSplitL "Hf"; first by iApply (wp_binop with "Hf") => //.
-  iIntros (w) "(-> & Hf)".
-  iApply (wp_if_true with "Hf").
-  {
-    unfold Wasm_int.Int32.modu.
-    simpl.
-    move => Hcontra.
-    apply Znumtheory.Zdivide_mod in Hdiv.
-    assert ((4 + length s * 4 < 65536)%Z) as Hsub.
-    { unfold two14 in Hsize. by lias. }
-    assert ((4 <= 4 + length s * 4)%Z) as Hslb.
-    { by lias. }
-    unfold Wasm_int.Int32.zero in Hcontra.
-    apply Wasm_int.Int32.repr_inv in Hcontra => //=.
-    { 
-      rewrite Wasm_int.Int32.Z_mod_modulus_eq in Hcontra.
-      unfold Wasm_int.Int32.modulus, Wasm_int.Int32.wordsize, Integers.Wordsize_32.wordsize in Hcontra.
-      rewrite <- Znumtheory.Zmod_div_mod in Hcontra => //; last by apply Znumtheory.Zmod_divide => //.
-      unfold two16 in Hdiv.
-      rewrite - Z.add_assoc in Hcontra.
-      rewrite Zplus_mod Hdiv Z.add_0_l in Hcontra.
-      rewrite Z.mod_mod in Hcontra => //.
-      rewrite Z.mod_small in Hcontra; first by lias.
-      split; by lias.
-    }
-    rewrite Wasm_int.Int32.Z_mod_modulus_eq.
-    unfold Wasm_int.Int32.modulus, Wasm_int.Int32.wordsize, Integers.Wordsize_32.wordsize.
-    rewrite <- Znumtheory.Zmod_div_mod => //; last by apply Znumtheory.Zmod_divide => //.
-    rewrite - Z.add_assoc.
-    rewrite Zplus_mod Hdiv Z.add_0_l.
-    rewrite Z.mod_mod => //.
-    remember (4 + length s * 4)%Z as x.
-    rewrite - Heqx.
-    split.
-    { 
-      assert ((0 <= x `mod` 65536)%Z); first by apply Z_mod_pos.
-      by lias.
-    }
-    assert ((x `mod` 65536 < 65536)%Z); first by apply Z_mod_lt.
-    replace (two_power_nat 32) with (4294967296)%Z => //.
-    by lias.
-  }
-  iIntros "!> Hf".
-  replace ([AI_basic (BI_block (Tf [] []) [])]) with ([] ++ [AI_basic (BI_block (Tf [] []) [])]) => //.
-  iApply (wp_block with "Hf") => //.
-  iIntros "!> Hf".
-  by iApply (wp_label_value with "Hf").
-Qed.
+  Context `{!wasmG Σ}.
   
-Lemma spec_push f0 n v (a : i32) s E :
-  ⊢ {{{ ⌜ f0.(f_inst).(inst_memory) !! 0 = Some n ⌝
-         ∗ ⌜ f0.(f_locs) !! 0 = Some (VAL_int32 a) ⌝ 
-         ∗ ⌜ f0.(f_locs) !! 1 = Some (value_of_int v) ⌝
-         ∗ ⌜ length f0.(f_locs) >= 3 ⌝
-         ∗ ⌜ (0 <= v <= Wasm_int.Int32.max_unsigned - 4 - S (length s) * 4 )%Z ⌝
-         ∗ ⌜ (length s < two14 - 1)%Z ⌝
-         ∗ isStack v s n
-         ∗ ↪[frame] f0 }}}
-    to_e_list push @ E
-    {{{ w, ⌜ w = immV [] ⌝ ∗
-           isStack v (a :: s) n ∗
-           ∃ f1, ↪[frame] f1 ∗ ⌜ f_inst f0 = f_inst f1 ⌝ }}}. 
-Proof.
-  iIntros "!>" (Φ) "(%Hinst & %Hloca & %Hlocv & %Hlocs & %Hv & %Hlens & Hstack & Hf) HΦ" => /=.
-  rewrite separate4.
-  iApply wp_seq.
-  instantiate (1 := λ x,  (⌜ x = immV [] ⌝ ∗ isStack v s n ∗ ↪[frame] f0)%I).
-  iSplitR; first by iIntros "(%H & _)".
-  iSplitL "Hstack Hf"; first by iApply (is_stack_valid with "[$Hstack $Hf]").
-  iIntros (w) "(-> & Hstack & Hf)".
-  simpl.
-  rewrite (separate1 (AI_basic _)).
-  iApply wp_seq.
-  instantiate (1 := λ x, (⌜ x = immV [value_of_int v] ⌝ ∗ ↪[frame] f0)%I).
-  iSplitR ; first by iIntros "[%Habs _]".
-  iSplitL "Hf".
-  - iApply (wp_get_local with "[] [$Hf]") => //=.
-  - iIntros (w) "[-> Hf]".
-    simpl.
-    rewrite separate2.
-    iApply wp_seq.
-    instantiate ( 1 := λ x, ((((⌜ x = immV [ value_of_int (v + 4 + length (s) * 4)%Z] ⌝
-                                           ∗ [∗ list] i↦w ∈  s,
-                                 N.of_nat n ↦[i32][ Z.to_N (v + 4 + length (s) * 4 - 4 - 4 * i)] w) ∗
+  Section code.
 
-                                                                                                    (∃ bs, ⌜ Z.of_nat (length bs) = (two16 - 4 - length s * 4)%Z ⌝ ∗ N.of_nat n↦[wms][Z.to_N (v + 4 + length s * 4)]bs)
-                                                                                            )
-                                ∗  N.of_nat n↦[wms][(Wasm_int.N_of_uint i32m (Wasm_int.int_of_Z i32m v) + N.zero)%N]bits (value_of_int (v + 4 + length (s) * 4)) )
-                               ∗ ↪[frame] f0)%I).
-    iSplitR ; first by iIntros "[[[[%Habs _] _] _] _]".
-    iDestruct "Hstack" as "(%Hdiv & %Hlen & Hv & Hs & Hrest)".
-    iSplitR "HΦ".
-  - iApply wp_load => //.
-    iSplitL "Hs Hrest".
-    iFrame.
-    done.
-    iFrame.
-    rewrite N.add_0_r.
-    iSimpl.
-    rewrite Wasm_int.Int32.Z_mod_modulus_eq.
-    rewrite Z.mod_small ; last by unfold Wasm_int.Int32.max_unsigned in Hv ; lia.
-    by iDestruct (i32_wms with "Hv") as "Hv" => //.
-  - iIntros (w) "[[[[->  Hs] Hrest] Hp] Hf]".
-    iSimpl.
-    iAssert (isStack v (s) n)%I with "[Hrest Hp Hs]" as "Hstack".
-    unfold isStack.
-    iFrame.
-    rewrite N.add_0_r.
-    simpl.
-    rewrite Wasm_int.Int32.Z_mod_modulus_eq.
-    rewrite Z.mod_small ; last by unfold Wasm_int.Int32.max_unsigned in Hv ; lia.
-    repeat iSplit => //=.
-    iApply i32_wms => //.
-  - rewrite separate2.
-    iApply (wp_seq _ _ _ (λ x, (⌜ x = immV [value_of_int (v + 4 + length s * 4)] ⌝
-                                           ∗ ↪[frame] _)%I)).
-    iSplitR ; first by iIntros "[%Habs _]".
-    iSplitL "Hf".
-  - iApply (wp_tee_local with "Hf").
-    iIntros "!> Hf".
-    rewrite separate1.
-    iApply wp_val_app => //.
-    iSplitR ; first by iIntros "!> [%Habs _]".
-    iApply (wp_set_local with "[] [$Hf]") => //=.
-  - iIntros (w) "[-> Hf]".
-    simpl.
+    Definition push_op :=
+      [BI_get_local 1 ;
+       BI_load T_i32 None N.zero N.zero ;
+       BI_tee_local 2 ;
+       i32const 65536;
+       BI_binop T_i32 (Binop_i (BOI_rem SX_U)) ;
+       BI_if (Tf [] []) [] [BI_unreachable] ;
+       BI_get_local 2 ;
+       BI_get_local 0 ;
+       BI_store T_i32 None N.zero N.zero ;
+       BI_get_local 1 ;
+       BI_get_local 2 ;
+       i32const 4 ;
+       BI_binop T_i32 (Binop_i BOI_add) ;
+       BI_store T_i32 None N.zero N.zero
+      ].
+        
+    Definition push :=
+      validate_stack 1 ++ push_op.
 
-    remember {| f_locs := set_nth (value_of_int (v + 4 + length s * 4))
-                                  (f_locs f0) 2 (value_of_int (v + 4 + length s * 4)) ;
-                f_inst := f_inst f0 |} as f1.
-    rewrite - Heqf1.
-    rewrite separate4.
-    iApply wp_seq.
-    instantiate (1 := λ x, (⌜ x = immV []⌝ ∗ ↪[frame] f1 )%I ).
-    iSplitR; first by iIntros "(%H & _)".
-    iSplitL "Hf"; first by iApply (push_not_full with "Hf") => //.
+  End code.
 
-    iIntros (w) "(-> & Hf)".
-    iSimpl.
+  Section specs.
 
-    rewrite (separate1 (AI_basic (BI_get_local 2))).
-    iApply wp_seq.
-    instantiate (1 := λ x, (⌜ x = immV [value_of_int (v + 4 + length s * 4)] ⌝ ∗ ↪[frame] f1)%I).
-    iSplitR; first by iIntros "(%H & _)".
-    iSplitL "Hf"; first iApply (wp_get_local with "[] [$Hf]") => //.
-    { rewrite Heqf1 => /=.
-        by rewrite set_nth_read. }
+    Lemma push_not_full v (s: list i32) f E:
+      (two16 | v)%Z ->  
+      (length s < two14 - 1)%Z ->
+      ↪[frame] f ⊢
+        WP [AI_basic (BI_const (value_of_int (v + 4 + length s * 4))); AI_basic (i32const 65536);
+            AI_basic (BI_binop T_i32 (Binop_i (BOI_rem SX_U))); AI_basic (BI_if (Tf [] []) [] [BI_unreachable])] @ E
+        {{ w, ⌜ w = immV [] ⌝ ∗ ↪[frame] f }}.
+    Proof.
+      move => Hdiv Hsize.
+      iIntros "Hf".
+      rewrite separate3.
+      iApply wp_seq.
+      instantiate (1 := λ w, (⌜ w = immV [ _ ]⌝ ∗ ↪[frame] f)%I).
+      iSplitR; first by iIntros "(%H & _)".
+      iSplitL "Hf"; first by iApply (wp_binop with "Hf") => //.
+      iIntros (w) "(-> & Hf)".
+      iApply (wp_if_true with "Hf").
+      {
+        unfold Wasm_int.Int32.modu.
+        simpl.
+        move => Hcontra.
+        apply Znumtheory.Zdivide_mod in Hdiv.
+        assert ((4 + length s * 4 < 65536)%Z) as Hsub.
+        { unfold two14 in Hsize. by lias. }
+        assert ((4 <= 4 + length s * 4)%Z) as Hslb.
+        { by lias. }
+        unfold Wasm_int.Int32.zero in Hcontra.
+        apply Wasm_int.Int32.repr_inv in Hcontra => //=.
+        { 
+          rewrite Wasm_int.Int32.Z_mod_modulus_eq in Hcontra.
+          unfold Wasm_int.Int32.modulus, Wasm_int.Int32.wordsize, Integers.Wordsize_32.wordsize in Hcontra.
+          rewrite <- Znumtheory.Zmod_div_mod in Hcontra => //; last by apply Znumtheory.Zmod_divide => //.
+          unfold two16 in Hdiv.
+          rewrite - Z.add_assoc in Hcontra.
+          rewrite Zplus_mod Hdiv Z.add_0_l in Hcontra.
+          rewrite Z.mod_mod in Hcontra => //.
+          rewrite Z.mod_small in Hcontra; first by lias.
+          split; by lias.
+        }
+        rewrite Wasm_int.Int32.Z_mod_modulus_eq.
+        unfold Wasm_int.Int32.modulus, Wasm_int.Int32.wordsize, Integers.Wordsize_32.wordsize.
+        rewrite <- Znumtheory.Zmod_div_mod => //; last by apply Znumtheory.Zmod_divide => //.
+        rewrite - Z.add_assoc.
+        rewrite Zplus_mod Hdiv Z.add_0_l.
+        rewrite Z.mod_mod => //.
+        remember (4 + length s * 4)%Z as x.
+        rewrite - Heqx.
+        split.
+        { 
+          assert ((0 <= x `mod` 65536)%Z); first by apply Z_mod_pos.
+          by lias.
+        }
+        assert ((x `mod` 65536 < 65536)%Z); first by apply Z_mod_lt.
+        replace (two_power_nat 32) with (4294967296)%Z => //.
+        by lias.
+      }
+      iIntros "!> Hf".
+      replace ([AI_basic (BI_block (Tf [] []) [])]) with ([] ++ [AI_basic (BI_block (Tf [] []) [])]) => //.
+      iApply (wp_block with "Hf") => //.
+      iIntros "!> Hf".
+      by iApply (wp_label_value with "Hf").
+    Qed.
+    
+    Lemma spec_op_push f0 n v (a : i32) s E :
+      ⊢ {{{ ⌜ f0.(f_inst).(inst_memory) !! 0 = Some n ⌝
+          ∗ ⌜ f0.(f_locs) !! 0 = Some (VAL_int32 a) ⌝ 
+          ∗ ⌜ f0.(f_locs) !! 1 = Some (value_of_int v) ⌝
+          ∗ ⌜ length f0.(f_locs) >= 3 ⌝
+          ∗ ⌜ (0 <= v <= Wasm_int.Int32.max_unsigned - 4 - S (length s) * 4 )%Z ⌝
+          ∗ ⌜ (length s < two14 - 1)%Z ⌝
+          ∗ isStack v s n
+          ∗ ↪[frame] f0 }}}
+        to_e_list push_op @ E
+        {{{ w, ⌜ w = immV [] ⌝ ∗
+                       isStack v (a :: s) n ∗
+                       ∃ f1, ↪[frame] f1 ∗ ⌜ f_inst f0 = f_inst f1 ⌝ }}}. 
+    Proof.
+      iIntros "!>" (Φ) "(%Hinst & %Hloca & %Hlocv & %Hlocs & %Hv & %Hlens & Hstack & Hf) HΦ" => /=.
+      simpl.
+      rewrite (separate1 (AI_basic _)).
+      iApply wp_seq.
+      instantiate (1 := λ x, (⌜ x = immV [value_of_int v] ⌝ ∗ ↪[frame] f0)%I).
+      iSplitR ; first by iIntros "[%Habs _]".
+      iSplitL "Hf".
+      - iApply (wp_get_local with "[] [$Hf]") => //=.
+      - iIntros (w) "[-> Hf]".
+        simpl.
+        rewrite separate2.
+        iApply wp_seq.
+        instantiate ( 1 := λ x, ((((⌜ x = immV [ value_of_int (v + 4 + length (s) * 4)%Z] ⌝
+                                            ∗ [∗ list] i↦w ∈  s,
+                                     N.of_nat n ↦[i32][ Z.to_N (v + 4 + length (s) * 4 - 4 - 4 * i)] w) ∗
 
-    iIntros (w) "(-> & Hf)".
-    simpl.
-    rewrite separate2.
-    iApply wp_seq.
-    instantiate (1 := λ x, (⌜ x = immV [value_of_int (v + 4 + length s * 4) ;
-                                        VAL_int32 a] ⌝ ∗ ↪[frame] f1)%I).
-    iSplitR ; first by iIntros "[%Habs _]".
-    iSplitL "Hf".
-  - rewrite separate1.
-    iApply wp_val_app => //.
-    iSplitR ; first by iIntros "!> [%Habs _]".
-    subst f1 ; iApply (wp_get_local with "[] [$Hf]") => //.
-    unfold set_nth.
-    destruct (f_locs f0) => //=.
-  - iIntros (w) "[-> Hf]".
-    iSimpl.
-    rewrite separate3.
-    iApply wp_seq.
-   instantiate
-      (1 := λ x, (((⌜ x = immV [] ⌝ ∗ N.of_nat n↦[i32][ Z.to_N v] Wasm_int.Int32.repr (v+4+length s * 4) ∗ ([∗ list] i↦w ∈ s, N.of_nat n↦[i32][Z.to_N (v + 4 + length s * 4 - 4 - 4 * i)] w) ∗ (∃ bs, ⌜ Z.of_nat (length bs) = (two16 - 4 - length (s) * 4 - 4)%Z ⌝ ∗ N.of_nat n↦[wms][Z.to_N (v + 4 + S (length s) * 4)]bs) )
-                     ∗ N.of_nat n ↦[wms][Wasm_int.N_of_uint i32m (Wasm_int.int_of_Z i32m (v + 4 + length s * 4)%Z) + N.zero]bits (VAL_int32 a)) ∗ ↪[frame] f1)%I).
-    iSplitR ; first by iIntros "[[[ %Habs _ ] _] _]". 
-    iDestruct "Hstack" as "(_ & _ & Hp & Hs & Hrest)".
-    iDestruct "Hrest" as (bs) "[%Hbs Hrest]".
-    unfold two16 in Hbs.
-    unfold two14 in Hlens.
-    remember (length s) as x.
-    do 4 (destruct bs ; first by exfalso ; clear Heqx s ; simpl in Hbs ; lia).
-    rewrite separate4.
-    unfold mem_block_at_pos at 1.
-    rewrite big_sepL_app.
-    iDestruct "Hrest" as "[Ha Hrest]".
-    iSplitR "HΦ".
-  - iApply wp_wand_r. iSplitL. iApply wp_store ; last first.
-    iFrame.
-    iSplitR "Ha".
-    iNext.
-    simpl.
-    subst x.
-    by instantiate (1 := λ x, (⌜ x = immV [] ⌝ ∗ N.of_nat n ↦[i32][ Z.to_N v] Wasm_int.Int32.repr (v + 4 + length s * 4) ∗ ([∗ list] i↦w ∈ s, N.of_nat n
-                           ↦[i32][ Z.to_N (v + 4 + length s * 4 - 4 - 4 * i)] w) ∗ ([∗ list] k↦y ∈ bs, N.of_nat n↦[wm][N.of_nat
-                                                 (N.to_nat
-                                                    (Z.to_N (v + 4 + length s * 4)) +
-                                                  S (S (S (S k))))]y))%I);
-    iFrame.
-    3: instantiate (1 := [b ; b0 ; b1 ; b2]) => //=. 
-    3: done.
-    2: subst f1 => //=.
-    iApply (big_sepL_impl with "Ha").
-    iIntros "!>" (k y) "% H".
-    rewrite of_nat_to_nat_plus.
-    simpl.
-    rewrite Wasm_int.Int32.Z_mod_modulus_eq Z.mod_small.
-    rewrite of_nat_to_nat_plus.
-    rewrite N.add_0_r.
-    by subst x.
-    unfold Wasm_int.Int32.max_unsigned in Hv.
-    rewrite - Heqx.
-    lia.
-    iIntros (w) "[[(-> & Hp & Hs & Hrest) Ha] Hf]".
-    iFrame.
-    iSplitR "Ha".
-    iSplit ; first done.
-    subst x ; iFrame.
-    iExists bs.
-    iSplit ; first iPureIntro.
-    simpl in Hbs.
-    remember (length s) as x.
-    rewrite - Heqx in Hbs.
-    unfold two16. lia.
-    iApply (big_sepL_impl with "Hrest").
-    iIntros "!>" (k x) "% H".
-    do 2 rewrite of_nat_to_nat_plus.
-    remember (length s) as y.
-    clear Heqy s.
-    replace (Z.to_N (v + 4 + y * 4) + N.of_nat (S (S (S (S k)))))%N with
-      (Z.to_N (v + 4 + S y * 4) + N.of_nat k)%N.
-    done.
-    lia.
-    by subst x.
-  - iIntros (w) "[[(-> & Hp & Hs & Hrest) Ha] Hf]".
-    unfold of_val, fmap, list_fmap.
-    iSimpl.
-    rewrite (separate1 (AI_basic _)).
-    iApply wp_seq.
-    instantiate (1 := λ x, ( ⌜ x = immV [value_of_int v] ⌝ ∗ ↪[frame]f1)%I).
-    iSplitR ; first by iIntros "[%Habs _]".
-    iSplitL "Hf".
-  - iApply (wp_get_local with "[] [$Hf]") => //.
-    subst f1 => //=.
-    unfold set_nth.
-    destruct (f_locs f0) => //=.
-    destruct l => //=.
-  - iIntros (w) "[-> Hf]".
-    unfold of_val, fmap, list_fmap.
-    iSimpl.
-    rewrite separate2.
-    iApply wp_seq.
-    instantiate (1 := λ x, ( ⌜ x = immV [value_of_int v ;
-                                         value_of_int ( v + 4 + length s * 4 ) ] ⌝
-                                        ∗ ↪[frame] f1)%I).
-    iSplitR ; first by iIntros "[%Habs _]".
-    iSplitL "Hf".
-  - rewrite separate1.
-    iApply wp_val_app => //.
-    iSplitR ; first by iIntros "!> [%Habs _]".
-    iApply (wp_get_local with "[] [$Hf]") => //.
-    subst f1 => //=.
-    rewrite set_nth_read => //=.
-    by subst x.
-  - iIntros (w) "[-> Hf]".
-    unfold of_val, fmap, list_fmap.
-    iSimpl.
-    rewrite separate4.
-    iApply wp_seq.
-    instantiate (1 := λ x, ( ⌜ x = immV [value_of_int v ;
-                                         value_of_int ( v + 4 + S (length s) * 4 )] ⌝
-                                        ∗ ↪[frame] f1)%I).
-    iSplitR ; first by iIntros "[%Habs _]".
-    iSplitL "Hf".
-  - rewrite separate1.
-    iApply wp_val_app => //.
-    iSplitR ; first by iIntros "!> [%Habs _]".
-    iApply (wp_binop with "Hf") => //=.
-    iPureIntro.
-    unfold Wasm_int.Int32.iadd, Wasm_int.Int32.add.
-    rewrite Wasm_int.Int32.unsigned_repr.
-    rewrite Wasm_int.Int32.unsigned_repr.
-    unfold value_of_int => //=.
-    rewrite - Heqx.
-    replace (v + 4 + x * 4 + 4)%Z with (v + 4 + S x * 4)%Z => //=.
-    lia.
-    unfold Wasm_int.Int32.max_unsigned, Wasm_int.Int32.modulus.
-    unfold Wasm_int.Int32.wordsize, Integers.Wordsize_32.wordsize.
-    replace (two_power_nat 32) with two32 ; last done.
-    unfold two32 ; lia.
-    rewrite - Heqx. lia.
-  - iIntros (w) "[-> Hf]".
-    unfold of_val, fmap, list_fmap.
-    iSimpl.
-    iApply wp_wand_r.
-    iSplitL "Hf Hp".
-  - iApply wp_store.
-    done.
-    instantiate (1 := bits (value_of_int (v + 4 + length s * 4))) => //=.
-    instantiate (2 := f1).
-    subst f1 => //=.
-    instantiate (1 := λ x, ⌜ x = immV [] ⌝%I).
-    iFrame.
-    iSplit => //=.
-    rewrite Wasm_int.Int32.Z_mod_modulus_eq.
-    rewrite Z.mod_small ; last by unfold Wasm_int.Int32.max_unsigned in Hv ; lia.
-    iDestruct (i32_wms with "Hp") as "Hp" => //.
-    rewrite N.add_0_r.
-    by subst x.
-  - iIntros (w) "[[-> Hp] Hf]".
-    iApply "HΦ".
-    iSplit => //=.
-    unfold isStack.
-    iSplitR "Hf".
-    repeat iSplit => //=.
-    iPureIntro ; rewrite - Heqx ; clear Heqx s ; unfold two14 ; lia.
-    iSplitL "Hp".
-    rewrite Wasm_int.Int32.Z_mod_modulus_eq.
-    rewrite Z.mod_small ; last by unfold Wasm_int.Int32.max_unsigned in Hv ; lia.
-    iApply i32_wms => //.
-    rewrite N.add_0_r.
-    unfold value_of_int => //=.
-    iSplitR "Hrest".
-    iSplitL "Ha".
-    iApply i32_wms => //.
-    rewrite Wasm_int.Int32.Z_mod_modulus_eq.
-    rewrite Z.mod_small ; last by unfold Wasm_int.Int32.max_unsigned in Hv ; lia.
-    rewrite N.add_0_r.
-    rewrite - Heqx.
-    replace (v + 4 + S x * 4 - 4 - 4 * 0%nat)%Z
-      with (v + 4 + x * 4)%Z ; last lia.
-    done.
-    iApply (big_sepL_impl with "Hs").
-    iIntros "!>" (k y) "%Hbits H".
-    rewrite - Heqx.
-    replace (v + 4 + S x * 4 - 4 - 4 * S k)%Z
-      with  (v + 4 + x * 4 - 4 - 4 * k)%Z ; last lia.
-    done.
-    iDestruct "Hrest" as (bs0) "[%Hbs0 Hrest]".
-    iExists bs0.
-    iSplit => //=.
-    iPureIntro.
-    rewrite - Heqx.
-    lia.
-    by subst x.
-    iExists _ ; by subst ; iFrame.
-Qed.
+                                     (∃ bs, ⌜ Z.of_nat (length bs) = (two16 - 4 - length s * 4)%Z ⌝ ∗ N.of_nat n↦[wms][Z.to_N (v + 4 + length s * 4)]bs)
+                                  )
+                                    ∗  N.of_nat n↦[wms][(Wasm_int.N_of_uint i32m (Wasm_int.int_of_Z i32m v) + N.zero)%N]bits (value_of_int (v + 4 + length (s) * 4)) )
+                                   ∗ ↪[frame] f0)%I).
+        iSplitR ; first by iIntros "[[[[%Habs _] _] _] _]".
+        iDestruct "Hstack" as "(%Hdiv & %Hlen & Hv & Hs & Hrest)".
+        iSplitR "HΦ".
+      - iApply wp_load => //.
+        iSplitL "Hs Hrest".
+        iFrame.
+        done.
+        iFrame.
+        rewrite N.add_0_r.
+        iSimpl.
+        rewrite Wasm_int.Int32.Z_mod_modulus_eq.
+        rewrite Z.mod_small ; last by unfold Wasm_int.Int32.max_unsigned in Hv ; lia.
+        by iDestruct (i32_wms with "Hv") as "Hv" => //.
+      - iIntros (w) "[[[[->  Hs] Hrest] Hp] Hf]".
+        iSimpl.
+        iAssert (isStack v (s) n)%I with "[Hrest Hp Hs]" as "Hstack".
+        unfold isStack.
+        iFrame.
+        rewrite N.add_0_r.
+        simpl.
+        rewrite Wasm_int.Int32.Z_mod_modulus_eq.
+        rewrite Z.mod_small ; last by unfold Wasm_int.Int32.max_unsigned in Hv ; lia.
+        repeat iSplit => //=.
+        iApply i32_wms => //.
+      - rewrite separate2.
+        iApply (wp_seq _ _ _ (λ x, (⌜ x = immV [value_of_int (v + 4 + length s * 4)] ⌝
+                                            ∗ ↪[frame] _)%I)).
+        iSplitR ; first by iIntros "[%Habs _]".
+        iSplitL "Hf".
+      - iApply (wp_tee_local with "Hf").
+        iIntros "!> Hf".
+        rewrite separate1.
+        iApply wp_val_app => //.
+        iSplitR ; first by iIntros "!> [%Habs _]".
+        iApply (wp_set_local with "[] [$Hf]") => //=.
+      - iIntros (w) "[-> Hf]".
+        simpl.
 
-End specs.
+        remember {| f_locs := set_nth (value_of_int (v + 4 + length s * 4))
+                                (f_locs f0) 2 (value_of_int (v + 4 + length s * 4)) ;
+                   f_inst := f_inst f0 |} as f1.
+        rewrite - Heqf1.
+        rewrite separate4.
+        iApply wp_seq.
+        instantiate (1 := λ x, (⌜ x = immV []⌝ ∗ ↪[frame] f1 )%I ).
+        iSplitR; first by iIntros "(%H & _)".
+        iSplitL "Hf"; first by iApply (push_not_full with "Hf") => //.
+
+        iIntros (w) "(-> & Hf)".
+        iSimpl.
+
+        rewrite (separate1 (AI_basic (BI_get_local 2))).
+        iApply wp_seq.
+        instantiate (1 := λ x, (⌜ x = immV [value_of_int (v + 4 + length s * 4)] ⌝ ∗ ↪[frame] f1)%I).
+        iSplitR; first by iIntros "(%H & _)".
+        iSplitL "Hf"; first iApply (wp_get_local with "[] [$Hf]") => //.
+        { rewrite Heqf1 => /=.
+          by rewrite set_nth_read. }
+
+        iIntros (w) "(-> & Hf)".
+        simpl.
+        rewrite separate2.
+        iApply wp_seq.
+        instantiate (1 := λ x, (⌜ x = immV [value_of_int (v + 4 + length s * 4) ;
+                                            VAL_int32 a] ⌝ ∗ ↪[frame] f1)%I).
+        iSplitR ; first by iIntros "[%Habs _]".
+        iSplitL "Hf".
+      - rewrite separate1.
+        iApply wp_val_app => //.
+        iSplitR ; first by iIntros "!> [%Habs _]".
+        subst f1 ; iApply (wp_get_local with "[] [$Hf]") => //.
+        unfold set_nth.
+        destruct (f_locs f0) => //=.
+      - iIntros (w) "[-> Hf]".
+        iSimpl.
+        rewrite separate3.
+        iApply wp_seq.
+        instantiate
+          (1 := λ x, (((⌜ x = immV [] ⌝ ∗ N.of_nat n↦[i32][ Z.to_N v] Wasm_int.Int32.repr (v+4+length s * 4) ∗ ([∗ list] i↦w ∈ s, N.of_nat n↦[i32][Z.to_N (v + 4 + length s * 4 - 4 - 4 * i)] w) ∗ (∃ bs, ⌜ Z.of_nat (length bs) = (two16 - 4 - length (s) * 4 - 4)%Z ⌝ ∗ N.of_nat n↦[wms][Z.to_N (v + 4 + S (length s) * 4)]bs) )
+                         ∗ N.of_nat n ↦[wms][Wasm_int.N_of_uint i32m (Wasm_int.int_of_Z i32m (v + 4 + length s * 4)%Z) + N.zero]bits (VAL_int32 a)) ∗ ↪[frame] f1)%I).
+        iSplitR ; first by iIntros "[[[ %Habs _ ] _] _]". 
+        iDestruct "Hstack" as "(_ & _ & Hp & Hs & Hrest)".
+        iDestruct "Hrest" as (bs) "[%Hbs Hrest]".
+        unfold two16 in Hbs.
+        unfold two14 in Hlens.
+        remember (length s) as x.
+        do 4 (destruct bs ; first by exfalso ; clear Heqx s ; simpl in Hbs ; lia).
+        rewrite separate4.
+        unfold mem_block_at_pos at 1.
+        rewrite big_sepL_app.
+        iDestruct "Hrest" as "[Ha Hrest]".
+        iSplitR "HΦ".
+      - iApply wp_wand_r. iSplitL. iApply wp_store ; last first.
+        iFrame.
+        iSplitR "Ha".
+        iNext.
+        simpl.
+        subst x.
+        by instantiate (1 := λ x, (⌜ x = immV [] ⌝ ∗ N.of_nat n ↦[i32][ Z.to_N v] Wasm_int.Int32.repr (v + 4 + length s * 4) ∗ ([∗ list] i↦w ∈ s, N.of_nat n
+                                                                                                                                                    ↦[i32][ Z.to_N (v + 4 + length s * 4 - 4 - 4 * i)] w) ∗ ([∗ list] k↦y ∈ bs, N.of_nat n↦[wm][N.of_nat
+                                                                                                                                                                                                                                                  (N.to_nat
+                                                                                                                                                                                                                                                     (Z.to_N (v + 4 + length s * 4)) +
+                                                                                                                                                                                                                                                     S (S (S (S k))))]y))%I);
+        iFrame.
+        3: instantiate (1 := [b ; b0 ; b1 ; b2]) => //=. 
+        3: done.
+        2: subst f1 => //=.
+        iApply (big_sepL_impl with "Ha").
+        iIntros "!>" (k y) "% H".
+        rewrite of_nat_to_nat_plus.
+        simpl.
+        rewrite Wasm_int.Int32.Z_mod_modulus_eq Z.mod_small.
+        rewrite of_nat_to_nat_plus.
+        rewrite N.add_0_r.
+        by subst x.
+        unfold Wasm_int.Int32.max_unsigned in Hv.
+        rewrite - Heqx.
+        lia.
+        iIntros (w) "[[(-> & Hp & Hs & Hrest) Ha] Hf]".
+        iFrame.
+        iSplitR "Ha".
+        iSplit ; first done.
+        subst x ; iFrame.
+        iExists bs.
+        iSplit ; first iPureIntro.
+        simpl in Hbs.
+        remember (length s) as x.
+        rewrite - Heqx in Hbs.
+        unfold two16. lia.
+        iApply (big_sepL_impl with "Hrest").
+        iIntros "!>" (k x) "% H".
+        do 2 rewrite of_nat_to_nat_plus.
+        remember (length s) as y.
+        clear Heqy s.
+        replace (Z.to_N (v + 4 + y * 4) + N.of_nat (S (S (S (S k)))))%N with
+          (Z.to_N (v + 4 + S y * 4) + N.of_nat k)%N.
+        done.
+        lia.
+        by subst x.
+      - iIntros (w) "[[(-> & Hp & Hs & Hrest) Ha] Hf]".
+        unfold of_val, fmap, list_fmap.
+        iSimpl.
+        rewrite (separate1 (AI_basic _)).
+        iApply wp_seq.
+        instantiate (1 := λ x, ( ⌜ x = immV [value_of_int v] ⌝ ∗ ↪[frame]f1)%I).
+        iSplitR ; first by iIntros "[%Habs _]".
+        iSplitL "Hf".
+      - iApply (wp_get_local with "[] [$Hf]") => //.
+        subst f1 => //=.
+        unfold set_nth.
+        destruct (f_locs f0) => //=.
+        destruct l => //=.
+      - iIntros (w) "[-> Hf]".
+        unfold of_val, fmap, list_fmap.
+        iSimpl.
+        rewrite separate2.
+        iApply wp_seq.
+        instantiate (1 := λ x, ( ⌜ x = immV [value_of_int v ;
+                                             value_of_int ( v + 4 + length s * 4 ) ] ⌝
+                                         ∗ ↪[frame] f1)%I).
+        iSplitR ; first by iIntros "[%Habs _]".
+        iSplitL "Hf".
+      - rewrite separate1.
+        iApply wp_val_app => //.
+        iSplitR ; first by iIntros "!> [%Habs _]".
+        iApply (wp_get_local with "[] [$Hf]") => //.
+        subst f1 => //=.
+        rewrite set_nth_read => //=.
+        by subst x.
+      - iIntros (w) "[-> Hf]".
+        unfold of_val, fmap, list_fmap.
+        iSimpl.
+        rewrite separate4.
+        iApply wp_seq.
+        instantiate (1 := λ x, ( ⌜ x = immV [value_of_int v ;
+                                             value_of_int ( v + 4 + S (length s) * 4 )] ⌝
+                                         ∗ ↪[frame] f1)%I).
+        iSplitR ; first by iIntros "[%Habs _]".
+        iSplitL "Hf".
+      - rewrite separate1.
+        iApply wp_val_app => //.
+        iSplitR ; first by iIntros "!> [%Habs _]".
+        iApply (wp_binop with "Hf") => //=.
+        iPureIntro.
+        unfold Wasm_int.Int32.iadd, Wasm_int.Int32.add.
+        rewrite Wasm_int.Int32.unsigned_repr.
+        rewrite Wasm_int.Int32.unsigned_repr.
+        unfold value_of_int => //=.
+        rewrite - Heqx.
+        replace (v + 4 + x * 4 + 4)%Z with (v + 4 + S x * 4)%Z => //=.
+        lia.
+        unfold Wasm_int.Int32.max_unsigned, Wasm_int.Int32.modulus.
+        unfold Wasm_int.Int32.wordsize, Integers.Wordsize_32.wordsize.
+        replace (two_power_nat 32) with two32 ; last done.
+        unfold two32 ; lia.
+        rewrite - Heqx. lia.
+      - iIntros (w) "[-> Hf]".
+        unfold of_val, fmap, list_fmap.
+        iSimpl.
+        iApply wp_wand_r.
+        iSplitL "Hf Hp".
+      - iApply wp_store.
+        done.
+        instantiate (1 := bits (value_of_int (v + 4 + length s * 4))) => //=.
+        instantiate (2 := f1).
+        subst f1 => //=.
+        instantiate (1 := λ x, ⌜ x = immV [] ⌝%I).
+        iFrame.
+        iSplit => //=.
+        rewrite Wasm_int.Int32.Z_mod_modulus_eq.
+        rewrite Z.mod_small ; last by unfold Wasm_int.Int32.max_unsigned in Hv ; lia.
+        iDestruct (i32_wms with "Hp") as "Hp" => //.
+        rewrite N.add_0_r.
+        by subst x.
+      - iIntros (w) "[[-> Hp] Hf]".
+        iApply "HΦ".
+        iSplit => //=.
+        unfold isStack.
+        iSplitR "Hf".
+        repeat iSplit => //=.
+        iPureIntro ; rewrite - Heqx ; clear Heqx s ; unfold two14 ; lia.
+        iSplitL "Hp".
+        rewrite Wasm_int.Int32.Z_mod_modulus_eq.
+        rewrite Z.mod_small ; last by unfold Wasm_int.Int32.max_unsigned in Hv ; lia.
+        iApply i32_wms => //.
+        rewrite N.add_0_r.
+        unfold value_of_int => //=.
+        iSplitR "Hrest".
+        iSplitL "Ha".
+        iApply i32_wms => //.
+        rewrite Wasm_int.Int32.Z_mod_modulus_eq.
+        rewrite Z.mod_small ; last by unfold Wasm_int.Int32.max_unsigned in Hv ; lia.
+        rewrite N.add_0_r.
+        rewrite - Heqx.
+        replace (v + 4 + S x * 4 - 4 - 4 * 0%nat)%Z
+          with (v + 4 + x * 4)%Z ; last lia.
+        done.
+        iApply (big_sepL_impl with "Hs").
+        iIntros "!>" (k y) "%Hbits H".
+        rewrite - Heqx.
+        replace (v + 4 + S x * 4 - 4 - 4 * S k)%Z
+          with  (v + 4 + x * 4 - 4 - 4 * k)%Z ; last lia.
+        done.
+        iDestruct "Hrest" as (bs0) "[%Hbs0 Hrest]".
+        iExists bs0.
+        iSplit => //=.
+        iPureIntro.
+        rewrite - Heqx.
+        lia.
+        by subst x.
+        iExists _ ; by subst ; iFrame.
+    Qed.
+
+    Lemma spec_push f0 n v (a : i32) s E :
+      ⊢ {{{ ⌜ f0.(f_inst).(inst_memory) !! 0 = Some n ⌝
+          ∗ ⌜ f0.(f_locs) !! 0 = Some (VAL_int32 a) ⌝ 
+          ∗ ⌜ f0.(f_locs) !! 1 = Some (value_of_int v) ⌝
+          ∗ ⌜ length f0.(f_locs) >= 3 ⌝
+          ∗ ⌜ (0 <= v <= Wasm_int.Int32.max_unsigned - 4 - S (length s) * 4 )%Z ⌝
+          ∗ ⌜ (length s < two14 - 1)%Z ⌝
+          ∗ isStack v s n
+          ∗ ↪[frame] f0 }}}
+        to_e_list push @ E
+        {{{ w, ⌜ w = immV [] ⌝ ∗
+                       isStack v (a :: s) n ∗
+                       ∃ f1, ↪[frame] f1 ∗ ⌜ f_inst f0 = f_inst f1 ⌝ }}}. 
+    Proof.
+      iIntros "!>" (Φ) "(%Hinst & %Hloca & %Hlocv & %Hlocs & %Hv & %Hlens & Hstack & Hf) HΦ" => /=.
+      rewrite separate4.
+      iApply wp_seq.
+      instantiate (1 := λ x,  (⌜ x = immV [] ⌝ ∗ isStack v s n ∗ ↪[frame] f0)%I).
+      iSplitR; first by iIntros "(%H & _)".
+      iSplitL "Hstack Hf"; first by iApply (is_stack_valid with "[$Hstack $Hf]").
+      iIntros (w) "(-> & Hstack & Hf) /=".
+      iApply (spec_op_push with "[$Hf $Hstack] [$]").
+      auto.
+    Qed.
+      
+  End specs.
 
 
 End stack.    
-      
+
